tests/elab/liftRflTactic.lean
@@ -1,0 +1,153 @@
+
+/-!
+# Tests of `lift_rfl`
+
+This file tests the `lift_rfl` tactic, a frontend to the `Lean.MVarId.liftReflToEq` meta tactic.
+-/
+
+-- For debugging:
+-- set_option trace.Meta.Tactic.relation true
+
+set_option pp.mvars.levels false
+set_option warn.sorry false
+
+/-! It is an error if it's already an equality. -/
+/--
+error: Tactic `liftReflToEq` failed: Goal is already an equality
+
+⊢ false = true
+-/
+#guard_msgs in
+example : false = true := by
+  lift_rfl
+
+/-! Unfolding abbrevations counts as progress, even if it's an equality. -/
+abbrev RevEq {α} (x y : α) := y = x
+/-- trace: ⊢ true = false -/
+#guard_msgs in
+example : RevEq false true := by
+  lift_rfl
+  trace_state
+  sorry
+
+/-! HEq is converted to Eq, if possible. -/
+/-- trace: ⊢ false = true -/
+#guard_msgs in
+example : false ≍ true := by
+  lift_rfl
+  trace_state
+  sorry
+
+/-! If HEq can't be converted, that's an error, since no progress is made. -/
+/--
+error: Tactic `liftReflToEq` failed: The left-hand side's type
+  Bool
+is not definitionally equal to the right-hand side's type
+  Nat
+
+⊢ false ≍ 2
+-/
+#guard_msgs in
+example : false ≍ 2 := by
+  lift_rfl
+
+/-!
+Type with reflexivity lemma
+-/
+inductive MyEq {α : Sort _} : α → α → Prop where
+  | rfl (x : α) : MyEq x x
+attribute [refl] MyEq.rfl
+
+/-- trace: ⊢ false = true -/
+#guard_msgs in
+example : MyEq false true := by
+  lift_rfl
+  trace_state
+  sorry
+
+/-!
+Heterogenous reflexivity, types first.
+-/
+inductive MyHEq1 : {α β : Sort _} → α → β → Prop where
+  | rfl {α} (x : α) : MyHEq1 x x
+attribute [refl] MyHEq1.rfl
+
+-- Lift to eq
+/-- trace: ⊢ false = true -/
+#guard_msgs in
+example : MyHEq1 false true := by
+  lift_rfl
+  trace_state
+  sorry
+
+-- Lift to HEq
+/-- trace: ⊢ false ≍ 2 -/
+#guard_msgs in
+example : MyHEq1 false 2 := by
+  lift_rfl
+  trace_state
+  sorry
+
+/-!
+Heterogenous reflexivity, types interlaced.
+-/
+inductive MyHEq2 : {α : Sort _} → α → {β : Sort _} → β → Prop where
+  | rfl {α} (x : α) : MyHEq2 x x
+attribute [refl] MyHEq2.rfl
+
+-- Lift to eq
+/-- trace: ⊢ false = true -/
+#guard_msgs in
+example : MyHEq2 false true := by
+  lift_rfl
+  trace_state
+  sorry
+
+-- Lift to HEq
+/-- trace: ⊢ false ≍ 2 -/
+#guard_msgs in
+example : MyHEq2 false 2 := by
+  lift_rfl
+  trace_state
+  sorry
+
+/-!
+Relation with proof obligations
+-/
+@[relation m n]
+def PosEq (m : Nat) (_ : m > 0) (n : Nat) (_ : n > 0) := m - n = n - m
+@[refl] theorem PosEq.rfl (m : Nat) (h : m > 0) : PosEq m h m h := Eq.refl (m - m)
+
+/--
+trace: m : Nat
+hm : m > 0
+n : Nat
+hn : n > 0
+⊢ m = n
+-/
+#guard_msgs in
+example (m : Nat) (hm : m > 0) (n : Nat) (hn : n > 0) : PosEq m hm n hn := by
+  lift_rfl
+  trace_state
+  sorry
+
+/-!
+Typeclasses are not currently supported.
+-/
+structure DecEquiv (α : Type u) (β : Type v) [DecidableEq α] [DecidableEq β] where
+  toFun : α → β
+  invFun : β → α
+@[refl] def DecEquiv.rfl (α : Type _) [DecidableEq α] : DecEquiv α α where
+  toFun := id
+  invFun := id
+/--
+error: Failed rewrite relation
+  DecEquiv (Fin n) (Fin m)
+to be reflexive. Unsolved goals
+case e_4
+m n : Nat
+⊢ instDecidableEqFin n ≍ instDecidableEqFin m
+-/
+#guard_msgs in
+example (m : Nat) (n : Nat) : DecEquiv (Fin n) (Fin m) := by
+  lift_rfl
